Updated early alloc example

linux/pkvm/early_alloc.c
@@ -3,27 +3,38 @@
  * Copyright (C) 2020 Google LLC
  * Author: Quentin Perret <qperret@google.com>
  */
+//#include <asm/kvm_pgtable.h>
+//
+//#include <nvhe/early_alloc.h>
+//#include <nvhe/memory.h>
 
 #include <asm/page-def.h>
 #include <stddef.h>
-#include <stdint.h>
 #include <refinedc.h>
-
 //@rc::import instances from refinedc.linux.pkvm.early_alloc (for proofs only)
+
+//struct kvm_pgtable_mm_ops hyp_early_alloc_mm_ops;
+//s64 __ro_after_init hyp_physvirt_offset;
+//
+//static unsigned long base;
+//static unsigned long end;
+//static unsigned long cur;
 
 struct
 [[rc::refined_by("base : loc", "given : Z", "remaining : Z")]]
 [[rc::let("z_cur : Z = {(base.2 + given * PAGE_SIZE)%Z}")]]
 [[rc::let("z_end : Z = {(base.2 + (given + remaining) * PAGE_SIZE)%Z}")]]
-[[rc::constraints("{0 ≤ given}", "{0 ≤ remaining}", "[alloc_global base]",
-				  "{base.2 + (given + remaining) * PAGE_SIZE <= max_int u64}")]]
+[[rc::constraints("{0 ≤ given}", "{0 ≤ remaining}", "[alloc_global base]")]]
+[[rc::constraints("{base.2 + (given + remaining) * PAGE_SIZE ≤ max_int u64}")]]
 region {
-  [[rc::field("z_end @ int<uintptr_t>")]] uintptr_t end;
-  [[rc::field("z_cur @ int<uintptr_t>")]] uintptr_t cur;
+  [[rc::field("z_end @ int<u64>")]]
+  unsigned long end;
+  [[rc::field("z_cur @ int<u64>")]]
+  unsigned long cur;
   [[rc::field("own_constrained<nonshr_constraint<"
                  "{(base.1, z_cur) ◁ₗ uninit (PAGES (Z.to_nat remaining))}>, "
-                 "base @ ptr<{Z.to_nat ((given + remaining) * PAGE_SIZE)}>>"
-                                      )]] unsigned char* base;
+                 "base @ intptr<u64>>")]]
+  unsigned long base;
 };
 
 static struct region mem;
@@ -32,20 +43,22 @@ static struct region mem;
 #define end (mem.end)
 #define cur (mem.cur)
 
+[[rc::parameters("p : loc", "n : Z")]]
+[[rc::args("&own<place<p>>", "{0} @ int<u8>", "n @ int<u64>")]]
+[[rc::requires("own p : uninit<{ly_with_align (Z.to_nat n) (Z.to_nat PAGE_SIZE)}>")]]
+[[rc::ensures("own p : zeroed<{ly_with_align (Z.to_nat n) (Z.to_nat PAGE_SIZE)}>")]]
+extern void memset(void *to, unsigned char c, unsigned long size);
+
 [[rc::parameters("base : loc", "given : Z", "remaining : Z")]]
 [[rc::requires("global mem : {(base, given, remaining)} @ region")]]
 [[rc::returns("given @ int<size_t>")]]
 [[rc::ensures("global mem : {(base, given, remaining)} @ region")]]
 [[rc::tactics("all: rewrite Z.add_simpl_l; try solve_goal.")]]
 [[rc::tactics("all: rewrite Z.shiftr_div_pow2 //= Z.div_mul //=.")]]
-size_t hyp_early_alloc_nr_pages(void){
-  return (cur - (uintptr_t) base) >> PAGE_SHIFT;
+unsigned long hyp_early_alloc_nr_used_pages(void)
+{
+  return (cur - base) >> PAGE_SHIFT;
 }
-
-[[rc::parameters("p : loc")]]
-[[rc::args("p @ &own<uninit<PAGE>>")]]
-[[rc::ensures("own p : zeroed<PAGE>")]]
-extern void clear_page(void *to);
 
 [[rc::parameters("base : loc", "given : Z", "remaining : Z", "n : Z")]]
 [[rc::args("n @ int<u32>")]]
@@ -55,56 +68,48 @@ extern void clear_page(void *to);
 [[rc::ensures("global mem : {(base, given + n, remaining - n)%Z} @ region")]]
 [[rc::tactics("all: try rewrite -> Z.shiftl_mul_pow2 in *; try lia.")]]
 [[rc::tactics("all: rewrite ?ly_offset_PAGES; try solve_goal.")]]
-void *hyp_early_alloc_contig(unsigned int nr_pages){
-  uintptr_t ret = cur, p;
-  unsigned int i;
+void *hyp_early_alloc_contig(unsigned int nr_pages)
+{
+  unsigned long size = (nr_pages << PAGE_SHIFT);
+  void *ret = copy_alloc_id(cur, (void*) base);
 
   if (!nr_pages)
     return NULL;
 
-  rc_unfold(base);
-  cur += nr_pages << PAGE_SHIFT;
-  if (cur > end) {
-    cur = ret;
+  if (end - cur < size)
     return NULL;
-  }
 
-  [[rc::exists("i : nat")]]
-  [[rc::inv_vars("i: i @ int<u32>")]]
-  [[rc::inv_vars("p: uninit<uintptr_t>")]]
-  [[rc::inv_vars("ret: {base.2 + given * PAGE_SIZE} @ int<uintptr_t>")]]
-  [[rc::constraints("[(base +ₗ given * PAGE_SIZE) ◁ₗ zeroed (PAGES i)]")]]
-  [[rc::constraints("[(base +ₗ (given + i) * PAGE_SIZE) ◁ₗ uninit (PAGES (Z.to_nat n - i)%nat)]")]]
-  [[rc::constraints("global mem : {(base, given + n, remaining - n)%Z} @ region")]]
-  [[rc::constraints("{i ≤ n}", "{0 ≤ given}")]]
-  for (i = 0; i < nr_pages; i++) {
-    rc_unfold(base);
-    p = ret + (i << PAGE_SHIFT);
-    clear_page(copy_alloc_id(p, base));
-  }
+  cur += size;
+  memset(ret, 0, size);
 
-  return copy_alloc_id(ret, base);
+  return ret;
 }
 
 [[rc::parameters("base : loc", "given : Z", "remaining : Z")]]
 [[rc::args("uninit<void*>")]]
 [[rc::requires("global mem : {(base, given, remaining)} @ region")]]
-[[rc::requires("{0 ≠ remaining}")]]
+[[rc::requires("{0 < remaining}")]]
 [[rc::returns("&own<zeroed<PAGE>>")]]
 [[rc::ensures("global mem : {(base, given + 1, remaining - 1)} @ region")]]
-void *hyp_early_alloc_page(void *arg){
-  rc_unfold(base);
+void *hyp_early_alloc_page(void *arg)
+{
   return hyp_early_alloc_contig(1);
 }
 
 [[rc::parameters("l : loc", "n : Z", "s : Z")]]
-[[rc::args("l @ &own<uninit<PAGES<{Z.to_nat n}>>>", "s @ int<u32>")]]
+[[rc::args("l @ &own<uninit<PAGES<{Z.to_nat n}>>>", "s @ int<u64>")]]
 [[rc::requires("{s = (n * PAGE_SIZE)%Z}", "[alloc_global l]")]]
 [[rc::requires("global mem : uninit<struct_region>")]]
 [[rc::ensures("global mem : {(l, 0, n)} @ region")]]
 [[rc::tactics("all: rewrite -> ly_size_PAGES in *; solve_goal.")]]
-void hyp_early_alloc_init(unsigned char* virt, unsigned int size){
-  base = virt;
-  end = (uintptr_t) ((uintptr_t) virt + size);
-  cur = (uintptr_t) virt;
+void hyp_early_alloc_init(void *virt, unsigned long size)
+{
+  //base = cur = (unsigned long)virt;
+  base = (unsigned long)virt;
+  cur = base;
+  end = base + size;
+
+  //hyp_early_alloc_mm_ops.zalloc_page = hyp_early_alloc_page;
+  //hyp_early_alloc_mm_ops.phys_to_virt = hyp_phys_to_virt;
+  //hyp_early_alloc_mm_ops.virt_to_phys = hyp_virt_to_phys;
 }
