linux/pkvm/proofs/early_alloc/generated_proof_hyp_early_alloc_contig.v
@@ -9,34 +9,20 @@ Section proof_hyp_early_alloc_contig.
   Context `{!typeG Σ} `{!globalG Σ}.
 
   (* Typing proof for [hyp_early_alloc_contig]. *)
-  Lemma type_hyp_early_alloc_contig (global_mem global_clear_page : loc) :
+  Lemma type_hyp_early_alloc_contig (global_mem global_memset : loc) :
     global_locs !! "mem" = Some global_mem →
-    global_clear_page ◁ᵥ global_clear_page @ function_ptr type_of_clear_page -∗
-    typed_function (impl_hyp_early_alloc_contig global_mem global_clear_page) type_of_hyp_early_alloc_contig.
+    global_memset ◁ᵥ global_memset @ function_ptr type_of_memset -∗
+    typed_function (impl_hyp_early_alloc_contig global_mem global_memset) type_of_hyp_early_alloc_contig.
   Proof.
     Open Scope printing_sugar.
-    start_function "hyp_early_alloc_contig" ([[[base given] remaining] n]) => arg_nr_pages local_i local_ret local_p.
+    start_function "hyp_early_alloc_contig" ([[[base given] remaining] n]) => arg_nr_pages local_size local_ret.
     split_blocks ((
-      <[ "#3" :=
-        ∃ i : nat,
-        arg_nr_pages ◁ₗ (n @ (int (u32))) ∗
-        local_i ◁ₗ (i @ (int (u32))) ∗
-        local_p ◁ₗ (uninit (uintptr_t)) ∗
-        local_ret ◁ₗ ((base.2 + given * PAGE_SIZE) @ (int (uintptr_t))) ∗
-        ((base +ₗ given * PAGE_SIZE) ◁ₗ zeroed (PAGES i)) ∗
-        ((base +ₗ (given + i) * PAGE_SIZE) ◁ₗ uninit (PAGES (Z.to_nat n - i)%nat)) ∗
-        (global_with_type "mem" Own (((base, given + n, remaining - n)%Z) @ (region))) ∗
-        ⌜i ≤ n⌝ ∗
-        ⌜0 ≤ given⌝
-    ]> $
       ∅
     )%I : gmap label (iProp Σ)) ((
       ∅
     )%I : gmap label (iProp Σ)).
     - repeat liRStep; liShow.
       all: print_typesystem_goal "hyp_early_alloc_contig" "#0".
-    - repeat liRStep; liShow.
-      all: print_typesystem_goal "hyp_early_alloc_contig" "#3".
     Unshelve. all: sidecond_hook; prepare_sideconditions; normalize_and_simpl_goal; try solve_goal; unsolved_sidecond_hook.
     all: try rewrite -> Z.shiftl_mul_pow2 in *; try lia.
     all: rewrite ?ly_offset_PAGES; try solve_goal.
