linux/pkvm/proofs/early_alloc/generated_proof_hyp_early_alloc_nr_used_pages.v
@@ -5,26 +5,26 @@ From refinedc.linux.pkvm.early_alloc Require Import instances.
 Set Default Proof Using "Type".
 
 (* Generated from [linux/pkvm/early_alloc.c]. *)
-Section proof_hyp_early_alloc_nr_pages.
+Section proof_hyp_early_alloc_nr_used_pages.
   Context `{!typeG Σ} `{!globalG Σ}.
 
-  (* Typing proof for [hyp_early_alloc_nr_pages]. *)
-  Lemma type_hyp_early_alloc_nr_pages (global_mem : loc) :
+  (* Typing proof for [hyp_early_alloc_nr_used_pages]. *)
+  Lemma type_hyp_early_alloc_nr_used_pages (global_mem : loc) :
     global_locs !! "mem" = Some global_mem →
-    ⊢ typed_function (impl_hyp_early_alloc_nr_pages global_mem) type_of_hyp_early_alloc_nr_pages.
+    ⊢ typed_function (impl_hyp_early_alloc_nr_used_pages global_mem) type_of_hyp_early_alloc_nr_used_pages.
   Proof.
     Open Scope printing_sugar.
-    start_function "hyp_early_alloc_nr_pages" ([[base given] remaining]).
+    start_function "hyp_early_alloc_nr_used_pages" ([[base given] remaining]).
     split_blocks ((
       ∅
     )%I : gmap label (iProp Σ)) ((
       ∅
     )%I : gmap label (iProp Σ)).
     - repeat liRStep; liShow.
-      all: print_typesystem_goal "hyp_early_alloc_nr_pages" "#0".
+      all: print_typesystem_goal "hyp_early_alloc_nr_used_pages" "#0".
     Unshelve. all: sidecond_hook; prepare_sideconditions; normalize_and_simpl_goal; try solve_goal; unsolved_sidecond_hook.
     all: rewrite Z.add_simpl_l; try solve_goal.
     all: rewrite Z.shiftr_div_pow2 //= Z.div_mul //=.
-    all: print_sidecondition_goal "hyp_early_alloc_nr_pages".
+    all: print_sidecondition_goal "hyp_early_alloc_nr_used_pages".
   Qed.
-End proof_hyp_early_alloc_nr_pages.
+End proof_hyp_early_alloc_nr_used_pages.
